trying to verify strcmp and selection sort, but still fail

init_db.js
@@ -40,7 +40,7 @@ function create_tables() {
 	basic_query("CREATE TABLE Requests (id INT AUTO_INCREMENT PRIMARY KEY, userID INT, event_name VARCHAR(255), event_date DATE, event_time TIME, event_deadline DATE, event_suburb VARCHAR(255), event_type VARCHAR(255), noPeople INT, qualityLevel VARCHAR(255), budget FLOAT(10,2), choice VARCHAR(255), additional_info VARCHAR(255), completed INT, FOREIGN KEY (userID) REFERENCES Users(id)) ", "created Requests table");
 	// not sure if foreign key is set up properly
 
-	basic_query("CREATE TABLE Businesses (id INT AUTO_INCREMENT PRIMARY KEY, title VARCHAR(255), userID INT, opening_hours VARCHAR(255), phone_no VARCHAR(20), email VARCHAR(255), description VARCHAR(255), FOREIGN KEY (userID) REFERENCES Users(id))", "created Businesses table");	// link userID to Users(id)
+	basic_query("CREATE TABLE Businesses (id INT AUTO_INCREMENT PRIMARY KEY, title VARCHAR(255), userID INT, opening_hours VARCHAR(255), phone_no VARCHAR(20), email VARCHAR(255), description VARCHAR(255), fame FLOAT(10,2), FOREIGN KEY (userID) REFERENCES Users(id))", "created Businesses table");	// link userID to Users(id)
 
 	basic_query("CREATE TABLE Bids(requestID INT, businessID INT, price FLOAT(10,2), comment VARCHAR(255), status TINYINT, FOREIGN KEY (requestID) REFERENCES Requests(id), FOREIGN KEY (businessID) REFERENCES Businesses(id), CONSTRAINT pk PRIMARY KEY(requestID, businessID)) ", "created Bids table");
 	// link businessID and reqID to Businesses(id) and Requests(id)
