alphabet_selection.dfy
@@ -1,56 +1,68 @@
-predicate StringEqual(a: String, b: String)
-requires a.Length == b.Length;
-{ forall i :: 0 <= i < a.Length ==> a[i] == b[i] }
+function method min(a: int, b: int): int
+{ if a <= b then a else b }
 
-predicate Sorted(a: array<String>, lo: int, hi: int)
-reads a;
-{ forall i, j :: lo <= i <= j < hi ==> strcmp(a[i], a[j]) <= 0 }
+predicate PrecedeEqual(a: string, b: string, n: int)
+requires n <= min(|a|, |b|);
+{ forall i :: 0 <= i < n ==> a[i] == b[i] }
 
-method strcmp(a: String, b: String) returns (res: int)
-requires a.Length <= b.Length;
-ensures res == 0 ==> StringEqual(a, b)
-ensures res < 0 ==> (a.Length <= b.Length && exists k :: 0 <= k < a.Length && a[k] < b[k] && forall i :: 0 <= i <= k ==> a[i] == b[i])
-ensures res > 0 ==> (a.Length <= b.Length && exists k :: 0 <= k < a.Length && a[k] > b[k] && forall i :: 0 <= i <= k ==> a[i] == b[i])
+//predicate StringEqual(a: string, b: string)
+//{ |a| == |b| && PrecedeEqual(a, b, |a|) }
+
+method strcmp(a: string, b: string) returns (res: int)
+ensures res == 0  ==> a == b;
+ensures res == -1 ==> (exists k :: 0 <= k < min(|a|, |b|) && a[k] < b[k] && PrecedeEqual(a, b, k)) || (|a| < |b| && PrecedeEqual(a, b, |a|));
+ensures res == 1  ==> (exists k :: 0 <= k < min(|a|, |b|) && a[k] > b[k] && PrecedeEqual(a, b, k)) || (|a| > |b| && PrecedeEqual(a, b, |b|));
 {
     var i := 0;
-    while (i < a.Length)
-    invariant 0 <= i <= a.Length;
-    invariant forall k :: 0 <= k < i ==> a[k] == b[k];
+    var minLen := min(|a|, |b|);
+    while (i < minLen)
+    invariant 0 <= i <= minLen;
+    invariant PrecedeEqual(a, b, i);
     {
-        if (a[k] < b[k]) { return -1; }
-        else if (a[k] > b[k]) {return 1; }
+        if (a[i] < b[i]) { return -1; }
+        else if (a[i] > b[i]) {return 1; }
         i := i + 1;
     }
-    return 0;
+    assert PrecedeEqual(a, b, min(|a|, |b|));
+    if (|a| < |b|) { return -1; }
+    else if (|a| > |b|) { return 1; }
+    else if (|a| == |b|) { return 0; }
 }
 
-method Sort(a: array<String>)
+////////////////////////////////////////////////////////////////////////////////
+predicate SmallerEqual(a: string, b: string)
+{ (exists k :: 0 <= k < min(|a|, |b|) && |a| < |b| && PrecedeEqual(a, b, k)) || (|a| < |b| && PrecedeEqual(a, b, |a|)) || a == b }
+
+predicate Sorted(a: array<string>, lo: int, hi: int)
+reads a;
+requires 0 <= lo && hi <= a.Length;
+{ forall i, j :: lo <= i <= j < hi ==> SmallerEqual(a[i], a[j]) }
+
+method Sort(a: array<string>)
 modifies a;
 requires a.Length > 1;
 ensures Sorted(a, 0, a.Length);
 ensures multiset(a[..]) == multiset(old(a)[..])
 {
-    var b: array<String> := new String[a.Length];
-    var min := a[0];
     var i := 0;
-    while (i < a.Length)
-    invariant 0 <= i <= a.Length;
-    invariant Sorted(b, 0, i);
+    while (i < a.Length - 1)
+    invariant 0 <= i < a.Length;
+    invariant Sorted(a, 0, i);
+    invariant multiset(a[..]) == multiset(old(a)[..]);
     {
-        var j := 0;
+        var j := i + 1;
+        var min_index := i;
         while (j < a.Length)
-        invariant 0 <= j <= a.Length;
+        invariant i < j <= a.Length;
+        invariant i <= min_index < a.Length;
+        invariant forall k :: i <= k < j ==> SmallerEqual(a[min_index], a[k]);
+        invariant forall k :: 0 <= k < i ==> SmallerEqual(a[k], a[min_index]);
         {
-            if (strcmp(min, a[j]) > 0) { min := a[j]; }
+            var cmp := strcmp(a[min_index], a[j]);
+            if (cmp > 0) { min_index := j; }
             j := j + 1;
         }
-        b[i] := min;
+        a[i], a[min_index] := a[min_index], a[i];
         i := i + 1;
     }
-}
-
-
-method Main()
-{
-
 }
