strcmp.dfy
@@ -1,0 +1,50 @@
+function method min(a: int, b: int): int
+{ if a <= b then a else b }
+
+predicate PrecedeEqual(a: string, b: string, n: int)
+requires n <= min(|a|, |b|);
+{ forall i :: 0 <= i < n ==> a[i] == b[i] }
+
+//predicate StringEqual(a: string, b: string)
+//{ |a| == |b| && PrecedeEqual(a, b, |a|) }
+
+method strcmp(a: string, b: string) returns (res: int)
+ensures res == 0  ==> a == b;
+ensures res == -1 ==> (exists k :: 0 <= k < min(|a|, |b|) && a[k] < b[k] && PrecedeEqual(a, b, k)) || (|a| < |b| && PrecedeEqual(a, b, |a|));
+ensures res == 1  ==> (exists k :: 0 <= k < min(|a|, |b|) && a[k] > b[k] && PrecedeEqual(a, b, k)) || (|a| > |b| && PrecedeEqual(a, b, |b|));
+{
+    var i := 0;
+    var minLen := min(|a|, |b|);
+    while (i < minLen)
+    invariant 0 <= i <= minLen;
+    invariant PrecedeEqual(a, b, i);
+    {
+        if (a[i] < b[i]) { return -1; }
+        else if (a[i] > b[i]) {return 1; }
+        i := i + 1;
+    }
+    assert PrecedeEqual(a, b, min(|a|, |b|));
+    if (|a| < |b|) { return -1; }
+    else if (|a| > |b|) { return 1; }
+    else if (|a| == |b|) { return 0; }
+}
+
+method Main() {
+  var a := "hello";
+  var b := "what";
+  var c := "hello";
+  
+  assert a == c;
+  var cmp := strcmp(a, c);
+  assert cmp == 0;
+  
+  assert a == "hello" && b == "what";
+  cmp := strcmp(a, b);
+  print "strcmp(", a, ",", b, ")=", cmp, '\n';
+  assert cmp == -1;
+  
+  assert a == "hello" && b == "what";
+  cmp := strcmp(b, a);
+  print "strcmp(", b, ",", a, ")=", cmp, '\n';
+  assert cmp == 1;
+}
